



COLUMBIA | ENGINEERING
The Fu Foundation School of Engineering and Applied Science

COLUMBIA UNIVERSITY

APMAE4302

METHODS IN COMPUTATIONAL SCIENCE

Homework 2

Author:

Matías I. Inostroza
(mii2106)

February 23, 2026

Contents

1	Problem 1	2
2	Problem 2	3

1 Problem 1

First, let's assume that there exist two problems described by:

$$\mathbf{A}\mathbf{u} = \mathbf{b} \quad \text{and} \quad \mathbf{A}\hat{\mathbf{u}} = \hat{\mathbf{b}} \quad (1)$$

By subtracting both:

$$\mathbf{A}\mathbf{u} - \mathbf{A}\hat{\mathbf{u}} = \mathbf{b} - \hat{\mathbf{b}} \quad (2)$$

$$\mathbf{A}(\mathbf{u} - \hat{\mathbf{u}}) = \mathbf{b} - \hat{\mathbf{b}} \quad (3)$$

$$\rightarrow (\mathbf{u} - \hat{\mathbf{u}}) = \mathbf{A}^{-1}(\mathbf{b} - \hat{\mathbf{b}}) \quad (4)$$

Considering $\|\mathbf{A}\mathbf{x}\| \leq \|\mathbf{A}\|\|\mathbf{x}\|$

$$\|\mathbf{A}(\mathbf{u} - \hat{\mathbf{u}})\| \leq \|\mathbf{A}\|\|\mathbf{u} - \hat{\mathbf{u}}\| = \|\mathbf{A}\|\|\mathbf{A}^{-1}(\mathbf{b} - \hat{\mathbf{b}})\| \leq \|\mathbf{A}\|\|\mathbf{A}^{-1}\|\|\mathbf{b} - \hat{\mathbf{b}}\| \quad (5)$$

Thus:

$$\|\mathbf{A}\|\|\mathbf{u} - \hat{\mathbf{u}}\| \leq \|\mathbf{A}\|\|\mathbf{A}^{-1}\|\|\mathbf{b} - \hat{\mathbf{b}}\| = \kappa(\mathbf{A})\|\mathbf{b} - \hat{\mathbf{b}}\| \quad (6)$$

Also, it can be established that $\|\mathbf{A}\mathbf{u}\| = \|\mathbf{b}\| \leq \|\mathbf{A}\|\|\mathbf{u}\|$, and therefore $\frac{\|\mathbf{b}\|}{\|\mathbf{u}\|} \leq \|\mathbf{A}\|$

By multiplying both by $\|\mathbf{u} - \hat{\mathbf{u}}\|$

$$\frac{\|\mathbf{b}\|}{\|\mathbf{u}\|}\|\mathbf{u} - \hat{\mathbf{u}}\| \leq \|\mathbf{A}\|\|\mathbf{u} - \hat{\mathbf{u}}\| \quad (7)$$

Therefore, by using equation 6 and equation 7:

$$\frac{\|\mathbf{b}\|}{\|\mathbf{u}\|}\|\mathbf{u} - \hat{\mathbf{u}}\| \leq \kappa(\mathbf{A})\|\mathbf{b} - \hat{\mathbf{b}}\| \quad (8)$$

$$\rightarrow \frac{\|\mathbf{u} - \hat{\mathbf{u}}\|}{\|\mathbf{u}\|} \leq \kappa(\mathbf{A}) \frac{\|\mathbf{b} - \hat{\mathbf{b}}\|}{\|\mathbf{b}\|} \quad (9)$$

2)

From equation 3:

$$\|\mathbf{A}(\mathbf{u} - \hat{\mathbf{u}})\| \leq \|\mathbf{A}\| \|\mathbf{u} - \hat{\mathbf{u}}\| \rightarrow \|\mathbf{r}\| \leq \|\mathbf{A}\| \|\mathbf{e}\| \quad (10)$$

And also as $\mathbf{u} = \mathbf{A}^{-1}\mathbf{b}$, then:

$$\|\mathbf{u}\| = \|\mathbf{A}^{-1}\mathbf{b}\| \leq \|\mathbf{A}^{-1}\| \|\mathbf{b}\| \quad (11)$$

By multiplying 10 by 11:

$$\|\mathbf{r}\| \|\mathbf{u}\| \leq \|\mathbf{A}^{-1}\| \|\mathbf{A}\| \|\mathbf{b}\| \|\mathbf{e}\| \quad (12)$$

$$\|\mathbf{r}\| \|\mathbf{u}\| \leq \kappa(\mathbf{A}) \|\mathbf{b}\| \|\mathbf{e}\| \quad (13)$$

$$\frac{1}{\kappa(\mathbf{A})} \frac{\|\mathbf{r}\|}{\|\mathbf{b}\|} \leq \frac{\|\mathbf{e}\|}{\|\mathbf{u}\|} \quad (14)$$

And as $\|\mathbf{e}\| = \|\mathbf{u} - \hat{\mathbf{u}}\|$ that means:

$$\frac{1}{\kappa(\mathbf{A})} \frac{\|\mathbf{r}\|}{\|\mathbf{b}\|} \leq \frac{\|\mathbf{e}\|}{\|\mathbf{u}\|} \leq \kappa(\mathbf{A}) \frac{\|\mathbf{r}\|}{\|\mathbf{b}\|} \quad (15)$$

2 Problem 2

If $\mathbf{v}_j = \sin(j\pi x_i)$ is an eigenvector of \mathbf{A} , it should happen that $\mathbf{A}\mathbf{v}_j = \lambda_i \mathbf{v}_j$

$$(\mathbf{A}\mathbf{v}_j)_i = \frac{1}{h^2}(-v^{i-1} + 2v^i - v^{i+1}) \quad (16)$$

$$= \frac{1}{h^2}(-\sin(j\pi(i-1)h) + 2\sin(j\pi(i)h) - \sin(j\pi(i+1)h)) \quad (17)$$

Lets redefine as the arguments as sums of angles $\theta = j\pi ih$ and $\phi = j\pi h$

$$\begin{aligned} (\mathbf{A}\mathbf{v}_j)_i &= \frac{1}{h^2}(-\sin(\theta - \phi) + 2\sin(\theta) - \sin(\theta + \phi)) \\ &= \frac{1}{h^2}(-\sin(\theta)\cos(\phi) + \sin(\phi)\cos(\theta) + 2\sin(\theta) - \sin(\theta)\cos(\phi) - \sin(\phi)\cos(\theta)) \\ &= \frac{1}{h^2}(-2\sin(\theta)\cos(\phi) + 2\sin(\theta)) \\ &= \frac{1}{h^2}(2\sin(\theta)(1 - \cos(\phi))) \end{aligned}$$

And $1 - \cos(\phi) = 2 \sin^2(\frac{\phi}{2})$

$$\begin{aligned} (\mathbf{A}\mathbf{v}_j)_i &= \frac{4}{h^2}(\sin^2(\frac{\phi}{2})) \sin(\theta) = \frac{4}{h^2}(\sin^2(\frac{j\pi h}{2})) \sin(j\pi i h) = \frac{4}{h^2}(\sin^2(\frac{j\pi h}{2})) \sin(j\pi x_i) \\ &= \frac{4}{h^2}(\sin^2(\frac{j\pi h}{2})) \mathbf{v}_j \end{aligned}$$

That $(\mathbf{A}\mathbf{v}_j)_i$ is the eigenvector of \mathbf{A}

2) The corresponding eigenvalue λ is the value in front of the eigenvector.

$$(\mathbf{A}\mathbf{v}_j)_i = \frac{4}{h^2}(\sin^2(\frac{j\pi h}{2})) \mathbf{v}_j = \lambda_j \mathbf{v}_j$$

Then:

$$\lambda_j = \frac{4}{h^2} \sin^2(\frac{j\pi h}{2}) = 4m^2 \sin^2(\frac{j\pi}{2m}) \quad (18)$$

For $j = 1, \dots, m-1$ (not including boundary conditions, where λ should be zero)

3) If $m \rightarrow \infty$:

- For $j=1$ is the lowest eigenvalue: $\frac{\pi}{2m}$ is small, then $\sin(\frac{\pi}{2m}) \approx \frac{\pi}{2m}$. Then

$$\lambda_{min} \approx 4m^2(\frac{\pi}{2m})^2 = \pi \quad (19)$$

- For $j=m-1$ is the lowest eigenvalue: $\frac{(m-1)\pi}{2m} = \frac{\pi}{2} - \frac{\pi}{2m} \approx \frac{\pi}{2}$, then $\sin(\frac{\pi}{2}) = 1$. Then:

$$\lambda_{max} \approx 4m^2(1)^2 = 4m^2 \quad (20)$$

Finally:

$$\kappa(\mathbf{A}) \approx \frac{4m}{\pi} = O(m^2) \quad (21)$$

3)

$$u(x) = \sin(k\pi x) + c(x - \frac{1}{2})^3 \quad (22)$$

$$u'(x) = k\pi \cos(k\pi x) + 3c(x - \frac{1}{2})^2 \quad (23)$$

$$u''(x) = -k^2\pi^2 \sin(k\pi x) + 6c(x - \frac{1}{2}) \quad (24)$$

Then, by substituting in $-u'' + \gamma u = f(x)$

$$k^2\pi^2 \sin(k\pi x) - 6c(x - \frac{1}{2}) + \gamma(\sin(k\pi x) + c(x - \frac{1}{2})^3) = f(x) \quad (25)$$

$$(k^2\pi^2 + \gamma) \sin(k\pi x) + \gamma c(x - \frac{1}{2})^3 - 6c(x - \frac{1}{2}) = f(x) \quad (26)$$